examples/opaque/client_proofs.v
@@ -1,5 +1,11 @@
+From stdpp Require Import base gmap.
 From mathcomp Require Import ssreflect.
-From iris.heap_lang Require Import proofmode.
+From iris.heap_lang Require Import notation proofmode.
+From iris.heap_lang.lib Require Import par.
+From cryptis Require Import lib term cryptis primitives tactics.
+
+From cryptis.examples Require Import alist.
+From cryptis.examples.opaque Require Import impl shared.
 
 Set Implicit Arguments.
 Unset Strict Implicit.
@@ -7,7 +13,64 @@ Unset Printing Implicit Defensive.
 
 Section Opaque.
 
-Context `{!heapGS Σ, !cryptisG Σ, !sessionG Σ}.
+Context `{!cryptisGS Σ, !heapGS Σ, !spawnG Σ}.
 Notation iProp := (iProp Σ).
 
-End Opaque.
+Lemma wp_client_session (uid c pw : term): 
+cryptis_ctx -∗
+channel c -∗
+public uid -∗
+WP Client.session uid c pw
+{{ x , True }}.
+Proof.
+  iIntros "#Cryptis #Hc #pubuid".
+  wp_lam. wp_pures.
+  wp_apply (wp_mk_nonce (fun _ => False)%I (fun _ => False)%I).
+  1: iAssumption.
+  iIntros "%x_u %Hnoncex_u #Hmintedx_u #Hprivatex_u #H!eqx_u Htokenx_u".
+  wp_pures.
+  wp_apply (wp_mk_nonce (fun _ => False)%I (fun _ => False)%I).
+  1: iAssumption.
+  iIntros "%r %Hnoncer #Hmintedr #Hprivater #H!eqr Htokenr".
+  wp_pures.
+  wp_apply wp_H'.
+  1: done.
+  iIntros "_".
+  unfold hash_result.
+  wp_apply wp_texp.
+  wp_pures.
+  wp_apply wp_texp.
+  wp_pures.
+  wp_list.
+  wp_term_of_list.
+  wp_pures.
+  do !rewrite subst_list_match /=.
+  wp_apply wp_send.
+  1: done.
+  do !rewrite public_of_list /=.
+  do !iSplit => //.
+  iApply public_TExp_iff.
+  intro contra.
+  destruct contra.
+  iRight.
+  do !iSplit => //.
+  iApply minted_THash.
+  iApply minted_tag.
+  admit.
+  iApply "H!eqr".
+  iNext. iModIntro.
+  admit.
+  iApply public_TExp.
+  by iApply public_g.
+  admit.
+  wp_pures.
+  wp_apply wp_recv.
+  1: done.
+  iIntros "%m2 #pubm2".
+  wp_list_of_term m2; wp_pures.
+  2: done.
+  wp_list_match => [β X_s envelope A_s | _].
+  2: by wp_pures.
+  intro Hm2eq.
+  wp_pures.
+Admitted.
