examples/opaque/server_proofs.v
@@ -1,5 +1,11 @@
+From stdpp Require Import base gmap.
 From mathcomp Require Import ssreflect.
-From iris.heap_lang Require Import proofmode.
+From iris.heap_lang Require Import notation proofmode.
+From iris.heap_lang.lib Require Import par.
+From cryptis Require Import lib term cryptis primitives tactics.
+
+From cryptis.examples Require Import alist.
+From cryptis.examples.opaque Require Import impl shared.
 
 Set Implicit Arguments.
 Unset Strict Implicit.
@@ -7,7 +13,100 @@ Unset Printing Implicit Defensive.
 
 Section Opaque.
 
-Context `{!heapGS Σ, !cryptisG Σ, !sessionG Σ}.
+Context `{!cryptisGS Σ, !heapGS Σ, !spawnG Σ}.
 Notation iProp := (iProp Σ).
+
+Lemma wp_server_session (db c : term) (alist : gmap term term): 
+cryptis_ctx -∗
+channel c -∗
+AList.is_alist db (repr <$> alist) -∗
+WP Server.session db c
+{{ x , True }}.
+Proof.
+  iIntros "#Cryptis #Hc Hdb".
+  wp_lam. wp_pures.
+  wp_apply (wp_recv with "Hc").
+  iIntros "%m1 #Hpubm1".
+  wp_list_of_term m1; wp_pures.
+  2: by iModIntro.
+  do !rewrite subst_list_match /=.
+  wp_list_match => [uid α X_u | _].
+  2: wp_pures; by iModIntro.
+  intro Hm1eq.
+  wp_bind (AList.find _ _).
+  iApply (AList.wp_find with "Hdb").
+  iIntros "!> Hdb". rewrite lookup_fmap.
+  case db_uid: (alist !! uid) => [file|]; wp_pures.
+  2: by iModIntro.
+  do !rewrite subst_list_match /=.
+  clear db_uid.
+  wp_list_of_term_eq file' e.
+  2: wp_pures.
+  2: by iModIntro.
+  wp_pures.
+  wp_list_match => [k_s p_s P_s P_u envelope _ | ].
+  2: intro H; wp_pures.
+  2: by iModIntro.
+  wp_apply (wp_mk_nonce (fun _ => False)%I (fun _ => False)%I).
+  1: iAssumption.
+  iIntros "%x_s %Hnoncex_s #Hmintedx_s #Hprivatex_s #H!eqx_s Htokenx_s".
+  wp_pures.
+  wp_apply wp_texp. wp_pures.
+  wp_apply wp_texp. wp_pures.
+  wp_apply wp_ke.
+  1: done.
+  iIntros "_".
+  wp_pures.
+  wp_list.
+  wp_apply wp_H.
+  1: done.
+  iIntros "_".
+  wp_pures.
+  unfold hash_result.
+  wp_list.
+  wp_apply wp_prf.
+  1: done.
+  iIntros "_".
+  wp_pures.
+  wp_list.
+  wp_apply wp_prf.
+  1: done.
+  iIntros "_".
+  unfold hash_result.
+  wp_list.
+  wp_term_of_list.
+  wp_pures.
+  rewrite Hm1eq.
+  rewrite public_of_list /=.
+  iDestruct "Hpubm1" as "[Hpubuid [Hpubα [HpubX_u _]]]".
+  wp_apply wp_send.
+  1: done.
+  1: do !rewrite public_of_list /=.
+  do !iSplit => //.
+  iApply public_TExp => //.
+  admit.
+  iApply public_TExp_iff.
+  intro contra. destruct contra.
+  iRight.
+  do !iSplit => //.
+  by iApply minted_TInt.
+  iApply "H!eqx_s". iNext. iModIntro. admit.
+  admit.
+  iApply public_THash.
+  admit.
+  wp_pures.
+  wp_apply (wp_recv with "Hc").
+  iIntros "%m3 #Hm3pub".
+  wp_pures.
+  wp_list.
+  wp_apply wp_prf => //.
+  iIntros "_".
+  wp_eq_term Heq; wp_pures.
+  2: by iModIntro.
+  wp_list.
+  wp_pures.
+  by iModIntro.
+Admitted.
+  
 
 End Opaque.
